LogicalRefinement/Denot/Wk.lean
@@ -6,40 +6,16 @@ import LogicalRefinement.Denot.Basic
 open AnnotSort
 open Annot
 
-theorem Term.denote_wk1_ty
+--TODO: make stricter...
+theorem Term.denote_wk1
   (A: Term) 
   (B: Term)
   (Γ: Context)
-  (x: B.stlc_ty.interp) 
+  (x: Option B.stlc_ty.interp) 
   (G: Γ.upgrade.stlc.interp) 
-  (a: A.stlc_ty.interp)
-  (a': A.wk1.stlc_ty.interp)
+  (a: Option A.stlc_ty.interp)
+  (a': Option A.wk1.stlc_ty.interp)
   (Haa': a' = A.stlc_ty_wk1 ▸ a)
-  (H: A.denote_ty' G a) 
-  : @denote_ty' A.wk1 ((Hyp.val B type)::Γ) (x, G) a'
-  := sorry
-  
-theorem Term.denote_wk1_prop
-  (A: Term) 
-  (φ: Term)
-  (Γ: Context)
-  (G: Γ.upgrade.stlc.interp) 
-  (a: A.stlc_ty.interp)
-  (a': A.wk1.stlc_ty.interp)
-  (Haa': a' = A.stlc_ty_wk1 ▸ a)
-  (H: @denote_ty' A Γ G a) 
-  : @denote_ty' A.wk1 ((Hyp.val φ prop)::Γ) G a'
-  := sorry
-  
-theorem Term.denote_wk1_gst
-  (A: Term) 
-  (B: Term)
-  (Γ: Context) 
-  (x: B.stlc_ty.interp)
-  (G: Γ.upgrade.stlc.interp) 
-  (a: A.stlc_ty.interp)
-  (a': A.wk1.stlc_ty.interp)
-  (Haa': a' = A.stlc_ty_wk1 ▸ a)
-  (H: A.denote_ty' G a) 
-  : @denote_ty' A.wk1 ((Hyp.gst B)::Γ) (x, G) a'
+  (H: A.denote_ty G a) 
+  : @denote_ty A.wk1 (B.stlc_ty::Γ.upgrade.stlc) (x, G) a'
   := sorry
